@prefix : <http://eis.iai.uni-bonn.de/semann/0.2/sdeo#> .
@prefix dc: <http://purl.org/dc/elements/1.1/> .
@prefix deo: <http://purl.org/spar/deo/> .
@prefix owl: <http://www.w3.org/2002/07/owl#> .
@prefix rdf: <http://www.w3.org/1999/02/22-rdf-syntax-ns#> .
@prefix sro: <http://salt.semanticauthoring.org/ontologies/sro#> .
@prefix xml: <http://www.w3.org/XML/1998/namespace> .
@prefix xsd: <http://www.w3.org/2001/XMLSchema#> .
@prefix rdfs: <http://www.w3.org/2000/01/rdf-schema#> .
@prefix terms: <http://purl.org/dc/terms/> .
@base <http://eis.iai.uni-bonn.de/semann/0.2/sdeo> .

<http://eis.iai.uni-bonn.de/semann/0.2/sdeo> rdf:type owl:Ontology ;
                                              
                                              dc:creator "Jaana Takis"^^xsd:string ;
                                              
                                              dc:description "Semann Discourse Elements Ontology (SDEO) is a vocabulary for the identification of the main elements of a scientific publication. As such it provides a convenient context reference for the later annotation of a document. SDEO uses the modified version of the Discourse Elements Ontology (in OWL 2 DL) that provides a structured vocabulary for rhetorical elements within documents (e.g. Introduction, Discussion, Acknowledgements, Reference List, Figures, Appendix), enabling these to be described in RDF.  It uses all the rhetorical block elements from the SALT Rhetorical Ontology (http://salt.semanticauthoring.org/ontologies/sro.rdfs) except 'Entities'."^^xsd:string ;
                                              
                                              dc:title "The Semann Discourse Elements Ontology (SDEO)"^^xsd:string ;
                                              
                                              rdfs:comment "This ontology describes the major elements of a scientific publication, especially rhetorical elements. The purpose of this ontology is to provide a context reference for the later annotation of a document within the Semann project."^^xsd:string ;
                                              
                                              dc:date "2014-10-14"@en ;
                                              
                                              dc:rights "This work is distributed under a Creative Commons Attribution License (http://creativecommons.org/licenses/by/3.0/)."@en .


#################################################################
#
#    Annotation properties
#
#################################################################


###  http://purl.org/dc/elements/1.1/creator

dc:creator rdf:type owl:AnnotationProperty .



###  http://purl.org/dc/elements/1.1/date

dc:date rdf:type owl:AnnotationProperty .



###  http://purl.org/dc/elements/1.1/description

dc:description rdf:type owl:AnnotationProperty .



###  http://purl.org/dc/elements/1.1/rights

dc:rights rdf:type owl:AnnotationProperty .



###  http://purl.org/dc/elements/1.1/title

dc:title rdf:type owl:AnnotationProperty .



###  http://www.w3.org/2000/01/rdf-schema#comment

rdfs:comment rdf:type owl:AnnotationProperty .



###  http://www.w3.org/2000/01/rdf-schema#label

rdfs:label rdf:type owl:AnnotationProperty .





#################################################################
#
#    Object Properties
#
#################################################################


###  http://purl.org/dc/terms/hasPart

terms:hasPart rdf:type owl:TransitiveProperty ;
              
              rdfs:label "has part"@en ;
              
              rdfs:comment "A related resource that is included either physically or logically in the described resource."@en ;
              
              owl:inverseOf terms:isPartOf ;
              rdfs:isDefinedBy <http://eis.iai.uni-bonn.de/semann/0.2/sdeo>;
              rdfs:subPropertyOf terms:relation .



###  http://purl.org/dc/terms/isPartOf

terms:isPartOf rdf:type owl:TransitiveProperty ;
               
               rdfs:label "is part of"@en ;
               
               rdfs:comment "A related resource in which the described resource is physically or logically included."@en ;
               rdfs:isDefinedBy <http://eis.iai.uni-bonn.de/semann/0.2/sdeo>;
               rdfs:subPropertyOf terms:relation .



###  http://purl.org/dc/terms/relation

terms:relation rdf:type owl:SymmetricProperty ;
               
               rdfs:label "has relation"@en ;
               
               rdfs:comment "A related resource."@en ;
               rdfs:isDefinedBy <http://eis.iai.uni-bonn.de/semann/0.2/sdeo>;
               rdfs:subPropertyOf owl:topObjectProperty .



###  http://www.w3.org/2002/07/owl#topObjectProperty

owl:topObjectProperty rdf:type owl:ObjectProperty .





#################################################################
#
#    Classes
#
#################################################################


###  http://eis.iai.uni-bonn.de/semann/0.2/sdeo#Author

<http://eis.iai.uni-bonn.de/semann/0.2/sdeo#Author> rdf:type owl:Class ;
                                                    
                                                    rdfs:label "author"@en ;
                                                    rdfs:isDefinedBy <http://eis.iai.uni-bonn.de/semann/0.2/sdeo>;
                                                    rdfs:comment "Author's name of the publication."@en .



###  http://eis.iai.uni-bonn.de/semann/0.2/sdeo#Keywords

<http://eis.iai.uni-bonn.de/semann/0.2/sdeo#Keywords> rdf:type owl:Class ;
                                                      
                                                      rdfs:label "keywords"@en ;
                                                      rdfs:isDefinedBy <http://eis.iai.uni-bonn.de/semann/0.2/sdeo>;
                                                      rdfs:comment "Key words and terms that describe the publication. Usually listed under a separate header in the publication."@en .



###  http://eis.iai.uni-bonn.de/semann/0.2/sdeo#Title

<http://eis.iai.uni-bonn.de/semann/0.2/sdeo#Title> rdf:type owl:Class ;
                                                   
                                                   rdfs:label "title"@en ;
                                                   rdfs:isDefinedBy <http://eis.iai.uni-bonn.de/semann/0.2/sdeo>;
                                                   rdfs:comment "Research publication's title."@en .



###  http://purl.org/spar/deo/Acknowledgements

deo:Acknowledgements rdf:type owl:Class ;
                     
                     rdfs:label "acknowledgements"@en ;
                     
                     rdfs:subClassOf deo:DiscourseElement ;
                     rdfs:isDefinedBy <http://eis.iai.uni-bonn.de/semann/0.2/sdeo>;
                     rdfs:comment "Usually part of the preface, or a separate section in its own right, often as part of the back matter, it acknowledges those, including funding agencies, who contributed to the undertaking of a research project described in a publication, or to the creation of the work in some way. In scientific articles, the acknowledgements are usually placed as a separated section immediately following the Discussion or Conclusions."@en .



###  http://purl.org/spar/deo/AuthorContribution

deo:AuthorContribution rdf:type owl:Class ;
                       
                       rdfs:label "author contribution"@en ;
                       
                       rdfs:subClassOf deo:DiscourseElement ;
                       rdfs:isDefinedBy <http://eis.iai.uni-bonn.de/semann/0.2/sdeo>;
                       rdfs:comment "A description of the roles played by an author in the publication."@en .



###  http://purl.org/spar/deo/BibliographicReference

deo:BibliographicReference rdf:type owl:Class ;
                           
                           rdfs:label "bibliographic reference"@en ;
                           
                           rdfs:subClassOf deo:Reference ;
                           rdfs:isDefinedBy <http://eis.iai.uni-bonn.de/semann/0.2/sdeo>;
                           rdfs:comment "A reference, usually contained in a footnote or a bibliographic reference list, that refer to another publication, such as a journal article, a book, a book chapter or a Web site. The inclusion of the bibliographic reference in a publication constitutes the performative act of bibliographic citation."@en .



###  http://purl.org/spar/deo/Biography

deo:Biography rdf:type owl:Class ;
              
              rdfs:label "biography"@en ;
              
              rdfs:subClassOf deo:DiscourseElement ;
              rdfs:isDefinedBy <http://eis.iai.uni-bonn.de/semann/0.2/sdeo>;
              rdfs:comment "Information describing a person and his or her life history and contributions."@en .



###  http://purl.org/spar/deo/Caption

deo:Caption rdf:type owl:Class ;
            
            rdfs:label "caption"@en ;
            
            rdfs:subClassOf deo:DiscourseElement ;
            rdfs:isDefinedBy <http://eis.iai.uni-bonn.de/semann/0.2/sdeo>;
            rdfs:comment "Text accompanying another item, such as a picture."@en .



###  http://purl.org/spar/deo/Data

deo:Data rdf:type owl:Class ;
         
         rdfs:label "data"@en ;
         
         rdfs:subClassOf deo:DiscourseElement ;
         rdfs:isDefinedBy <http://eis.iai.uni-bonn.de/semann/0.2/sdeo>;
         rdfs:comment "A textual description of data used or produced in the work which the document describes, or the data themselves."@en .



###  http://purl.org/spar/deo/DatasetDescription

deo:DatasetDescription rdf:type owl:Class ;
                       
                       rdfs:label "dataset description"@en ;
                       
                       rdfs:subClassOf deo:ExternalResourceDescription ;
                       rdfs:isDefinedBy <http://eis.iai.uni-bonn.de/semann/0.2/sdeo>;
                       rdfs:comment "Information describing a dataset held in an external database or repository and including a reference to it, such as a database ID or an accession number."@en .



###  http://purl.org/spar/deo/Dedication

deo:Dedication rdf:type owl:Class ;
               
               rdfs:label "dedication"@en ;
               
               rdfs:subClassOf deo:DiscourseElement ;
               rdfs:isDefinedBy <http://eis.iai.uni-bonn.de/semann/0.2/sdeo>;
               rdfs:comment "Text in which the author names the person or people for whom he/she has written the document, or to whose memory it is dedicated."@en .



###  http://purl.org/spar/deo/DiscourseElement

deo:DiscourseElement rdf:type owl:Class ;
                     
                     rdfs:label "discourse element"@en ;
                     
                     rdfs:subClassOf owl:Thing ;
                     rdfs:isDefinedBy <http://eis.iai.uni-bonn.de/semann/0.2/sdeo>;
                     rdfs:comment "An element of a document that carries out a rhetorical function."@en .



###  http://purl.org/spar/deo/Epilogue

deo:Epilogue rdf:type owl:Class ;
             
             rdfs:label "epilogue"@en ;
             
             rdfs:subClassOf deo:DiscourseElement ;
             rdfs:isDefinedBy <http://eis.iai.uni-bonn.de/semann/0.2/sdeo>;
             rdfs:comment "A piece of writing at the end of a work of literature or drama, usually used to bring closure to the work."@en .



###  http://purl.org/spar/deo/ExternalResourceDescription

deo:ExternalResourceDescription rdf:type owl:Class ;
                                
                                rdfs:label "external resource description"@en ;
                                
                                rdfs:subClassOf [ rdf:type owl:Class ;
                                                  owl:intersectionOf ( deo:DiscourseElement
                                                                       [ rdf:type owl:Restriction ;
                                                                         owl:onProperty terms:hasPart ;
                                                                         owl:someValuesFrom deo:Reference
                                                                       ]
                                                                     )
                                                ] ;
                                rdfs:isDefinedBy <http://eis.iai.uni-bonn.de/semann/0.2/sdeo>;
                                rdfs:comment "Information describing an external resource and including a reference to that resource."@en .



###  http://purl.org/spar/deo/FutureWork

deo:FutureWork rdf:type owl:Class ;
               
               rdfs:label "future work"@en ;
               
               rdfs:subClassOf deo:DiscourseElement ;
               rdfs:isDefinedBy <http://eis.iai.uni-bonn.de/semann/0.2/sdeo>;
               rdfs:comment "A proposal for new investigation to be undertaken in order to continue and advance the work described in the publication."@en .



###  http://purl.org/spar/deo/Introduction

deo:Introduction rdf:type owl:Class ;
                 
                 rdfs:label "introduction"@en ;
                 
                 rdfs:subClassOf deo:DiscourseElement ;
                 rdfs:isDefinedBy <http://eis.iai.uni-bonn.de/semann/0.2/sdeo>;
                 rdfs:comment "An initial description which states the purpose and goals of the following writing, and, in the case of journal articles, typically includes background information on the research topic and a review of related work in the area."@en .



###  http://purl.org/spar/deo/Legend

deo:Legend rdf:type owl:Class ;
           
           rdfs:label "legend"@en ;
           
           rdfs:subClassOf deo:Caption ;
           rdfs:isDefinedBy <http://eis.iai.uni-bonn.de/semann/0.2/sdeo>;
           rdfs:comment "Informative text that explicitly explains another item, such as a figure or a table."@en .



###  http://purl.org/spar/deo/Materials

deo:Materials rdf:type owl:Class ;
              
              rdfs:label "materials"@en ;
              
              rdfs:subClassOf deo:DiscourseElement ;
              rdfs:isDefinedBy <http://eis.iai.uni-bonn.de/semann/0.2/sdeo>;
              rdfs:comment "A description in a research paper documenting the specialized materials used in the work described. This description is often combined with a description of the methods used, in a section entitled 'Methods and Materials', 'Experimental' or a related term."@en .



###  http://purl.org/spar/deo/Methods

deo:Methods rdf:type owl:Class ;
            
            rdfs:label "methods"@en ;
            
            rdfs:subClassOf deo:DiscourseElement ;
            rdfs:isDefinedBy <http://eis.iai.uni-bonn.de/semann/0.2/sdeo>;
            rdfs:comment "A description in a research paper documenting the specialized methods used in the work described. This description is often combined with a description of the materials used, in a section entitled 'Methods and Materials', 'Experimental' or a related term."@en .



###  http://purl.org/spar/deo/Model

deo:Model rdf:type owl:Class ;
          
          rdfs:label "model"@en ;
          
          rdfs:subClassOf deo:DiscourseElement ;
          rdfs:isDefinedBy <http://eis.iai.uni-bonn.de/semann/0.2/sdeo>;
          rdfs:comment "A description of a model used or produced by the work described in the publication."@en .



###  http://purl.org/spar/deo/Postscript

deo:Postscript rdf:type owl:Class ;
               
               rdfs:label "postscript"@en ;
               
               rdfs:subClassOf deo:DiscourseElement ;
               rdfs:isDefinedBy <http://eis.iai.uni-bonn.de/semann/0.2/sdeo>;
               rdfs:comment "Text added after the signature of a letter, or sometimes after the main body of an essay or book."@en .



###  http://purl.org/spar/deo/ProblemStatement

deo:ProblemStatement rdf:type owl:Class ;
                     
                     rdfs:label "problem statement"@en ;
                     
                     rdfs:subClassOf deo:DiscourseElement ;
                     rdfs:isDefinedBy <http://eis.iai.uni-bonn.de/semann/0.2/sdeo>;
                     rdfs:comment "A concise description of the issues that needed to be addressed by a work described in the document."@en .



###  http://purl.org/spar/deo/Prologue

deo:Prologue rdf:type owl:Class ;
             
             rdfs:label "prologue"@en ;
             
             rdfs:subClassOf deo:DiscourseElement ;
             rdfs:isDefinedBy <http://eis.iai.uni-bonn.de/semann/0.2/sdeo>;
             rdfs:comment "A piece of writing at the beginning of a work of literature or drama, usually used to set the scene or to introduce the work."@en .



###  http://purl.org/spar/deo/Reference

deo:Reference rdf:type owl:Class ;
              
              rdfs:label "reference"@en ;
              
              rdfs:subClassOf deo:DiscourseElement ;
              rdfs:isDefinedBy <http://eis.iai.uni-bonn.de/semann/0.2/sdeo>;
              rdfs:comment "A reference to a specific part of the document, or to another publication."@en .



###  http://purl.org/spar/deo/RelatedWork

deo:RelatedWork rdf:type owl:Class ;
                
                rdfs:label "related work"@en ;
                
                rdfs:subClassOf deo:DiscourseElement ;
                rdfs:isDefinedBy <http://eis.iai.uni-bonn.de/semann/0.2/sdeo>;
                rdfs:comment "The authors' critical review of current knowledge by specific reference to others' work, both in terms of substantive findings and theoretical and methodological contributions to a particular topic. This description is often included within the introduction section."@en .



###  http://purl.org/spar/deo/Results

deo:Results rdf:type owl:Class ;
            
            rdfs:label "results"@en ;
            
            rdfs:subClassOf deo:DiscourseElement ;
            rdfs:isDefinedBy <http://eis.iai.uni-bonn.de/semann/0.2/sdeo>;
            rdfs:comment "The report of the specific findings of an investigation, given without discussion or conclusion being drawn."@en .



###  http://purl.org/spar/deo/SupplementaryInformationDescription

deo:SupplementaryInformationDescription rdf:type owl:Class ;
                                        
                                        rdfs:label "supplementary information description"@en ;
                                        
                                        rdfs:subClassOf deo:ExternalResourceDescription ;
                                        rdfs:isDefinedBy <http://eis.iai.uni-bonn.de/semann/0.2/sdeo>;
                                        rdfs:comment "Information describing supplementary information relating to the document, including references or links to the relevant supplementary information."@en .
                                        

###  http://salt.semanticauthoring.org/ontologies/sro#Abstract

sro:Abstract rdf:type owl:Class ;
                                                      
                                                      rdfs:label "abstract"@en ;
                                                      rdfs:subClassOf deo:DiscourseElement ;
                                                      rdfs:isDefinedBy <http://eis.iai.uni-bonn.de/semann/0.2/sdeo>;
                                                      rdfs:comment "A brief summary of a research publication or any in-depth analysis of a particular subject or discipline, the purpose of which is to help the reader quickly ascertain the publication's purpose."@en .
                                                      

###  http://salt.semanticauthoring.org/ontologies/sro#Background

sro:Background rdf:type owl:Class ;
               
               rdfs:label "background"@en ;
               
               rdfs:subClassOf deo:DiscourseElement ;
               rdfs:isDefinedBy <http://eis.iai.uni-bonn.de/semann/0.2/sdeo>;
               rdfs:comment "Presentation of information that is essential for understanding the situation or problem that is the subject of the publication. In a journal article, the background is usually part of the Introduction, but may be present as separated section."@en .



###  http://salt.semanticauthoring.org/ontologies/sro#Conclusion

sro:Conclusion rdf:type owl:Class ;
               
               rdfs:label "conclusion"@en ;
               
               rdfs:subClassOf deo:DiscourseElement ;
               rdfs:isDefinedBy <http://eis.iai.uni-bonn.de/semann/0.2/sdeo>;
               rdfs:comment "A reflection on the preceding text, summarizing the evidence, arguments or premises presented in the document and their logical outcomes. Conclusions are a fundamental feature in academic research publications, and may be included in the Discussion section."@en .



###  http://salt.semanticauthoring.org/ontologies/sro#Contribution

sro:Contribution rdf:type owl:Class ;
                 
                 rdfs:label "contribution"@en ;
                 
                 rdfs:subClassOf deo:DiscourseElement ;
                 rdfs:isDefinedBy <http://eis.iai.uni-bonn.de/semann/0.2/sdeo>;
                 rdfs:comment "A description of the part that this publication plays in the overall field."@en .



###  http://salt.semanticauthoring.org/ontologies/sro#Discussion

sro:Discussion rdf:type owl:Class ;
               
               rdfs:label "discussion"@en ;
               
               rdfs:subClassOf deo:DiscourseElement ;
               rdfs:isDefinedBy <http://eis.iai.uni-bonn.de/semann/0.2/sdeo>;
               rdfs:comment "An interpretation and discussion of the results obtained and an analysis of their significance, in support of conclusions. These conclusions may be part of this discussion or may be included in a separate section of the document."@en .



###  http://salt.semanticauthoring.org/ontologies/sro#Evaluation

sro:Evaluation rdf:type owl:Class ;
               
               rdfs:label "evaluation"@en ;
               
               rdfs:subClassOf deo:DiscourseElement ;
               rdfs:isDefinedBy <http://eis.iai.uni-bonn.de/semann/0.2/sdeo>;
               rdfs:comment "A consideration of the value, meaning and significance of the results obtained."@en .



###  http://salt.semanticauthoring.org/ontologies/sro#Motivation

sro:Motivation rdf:type owl:Class ;
               
               rdfs:label "motivation"@en ;
               
               rdfs:subClassOf deo:DiscourseElement ;
               rdfs:isDefinedBy <http://eis.iai.uni-bonn.de/semann/0.2/sdeo>;
               rdfs:comment "A description of the justification for undertaking the work described in the publication."@en .



###  http://salt.semanticauthoring.org/ontologies/sro#Scenario

sro:Scenario rdf:type owl:Class ;
             
             rdfs:label "scenario"@en ;
             
             rdfs:subClassOf deo:DiscourseElement ;
             rdfs:isDefinedBy <http://eis.iai.uni-bonn.de/semann/0.2/sdeo>;
             rdfs:comment "A presentation of a use case or test, based on a real or hypothetical situation, used to help someone think through a complex problem or system."@en .



###  http://www.w3.org/2002/07/owl#Thing

owl:Thing rdf:type owl:Class .




###  Generated by the OWL API (version 3.4.2) http://owlapi.sourceforge.net

